theories/Spilling/RegisterBound.v
@@ -9,25 +9,6 @@ Require Import ReconstrLiveG ToBeOutsourced.
 Set Implicit Arguments.
 (* TODO: outsource *)
 
-
-
-
-Definition reconstr_live_do_spill
-           (slot : var -> var)
-           (Λ : list (⦃var⦄ * ⦃var⦄))
-           (ZL : list params)
-           (G : ⦃var⦄)
-           (s : stmt)
-           (sl : spilling)
-  : ann ⦃var⦄
-  :=
-    reconstr_live (slot_merge slot Λ)
-                  ((slot_lift_params slot) ⊜ Λ ZL)
-                  G
-                  (do_spill slot s sl (compute_ib ⊜ ZL Λ))
-                  (do_spill_rm slot sl)
-.
-
 Lemma union_empty_r
       (X : Type)
       `{OrderedType X}
