theories/Spilling/SpillSim.v
@@ -1,0 +1,175 @@
+Require Import CSet Util Fresh Filter Take MoreList OUnion AllInRel MapDefined.
+Require Import IL Annotation LabelsDefined Liveness TrueLiveness SimI.
+Require Import RenamedApart.
+Require Import SetUtil Spilling ReconstrLive DoSpill ReconstrLiveUtil.
+
+Set Implicit Arguments.
+Unset Printing Records.
+
+Section Correctness.
+
+  Variable slot : var -> var.
+
+
+Instance SR : PointwiseProofRelationI (((set var) * (set var)) * params) := {
+   ParamRelIP RMZ Z Z' := Z' = slot_lift_params slot (fst RMZ) Z /\ Z = snd RMZ;
+   ArgRelIP V V' RMZ VL VL' :=
+     VL' = extend_args VL' (mark_elements (snd RMZ) (fst (fst RMZ) ∩ snd (fst RMZ)))
+}.
+
+Smpl Add match goal with
+         | [ |- context [ ❬@lookup_list ?X ?Y ?f ?L❭ ] ] =>
+           rewrite (@lookup_list_length X Y f L)
+         end : len.
+
+Lemma lookup_list_map X Y (f:X->Y) L
+  : lookup_list f L = f ⊝ L.
+Proof.
+  induction L; simpl; f_equal; eauto.
+Qed.
+
+
+Lemma injective_unique X `{OrderedType X} Y `{OrderedType Y} (f:X->Y) `{ Proper _ (_eq ==> _eq) f} xl
+  : injective_on (of_list xl) f
+    -> unique xl -> unique (lookup_list f xl).
+Proof.
+  intros Inj Uniq.
+  general induction xl; simpl in *; dcr; eauto.
+  - split; eauto using injective_on_incl with cset.
+    rewrite InA_in. rewrite InA_in in H2.
+    intro.
+    rewrite of_list_lookup_list in H4; eauto.
+    eapply lookup_set_spec in H4; eauto; dcr.
+    exploit Inj; eauto; cset_tac.
+Qed.
+
+Lemma injective_unique_map X `{OrderedType X} Y `{OrderedType Y} (f:X->Y) `{ Proper _ (_eq ==> _eq) f} xl
+  : injective_on (of_list xl) f
+    -> unique xl -> unique (f ⊝ xl).
+Proof.
+  rewrite <- lookup_list_map; eauto using injective_unique.
+Qed.
+
+
+Lemma sim_write_moves r L V s L' V' s' xl yl (Len:❬xl❭ = ❬yl❭)
+  : (forall D (V'':onv val), agree_on eq D (V'[xl <-- lookup_list V' yl]) V''
+                        -> paco3 (sim_gen (S':=I.state)) r Sim (L, V, s) (L', V'', s'))
+    -> defined_on (of_list yl) V'
+    -> disj (of_list xl) (of_list yl)
+    -> unique xl
+    -> paco3 (sim_gen (S':=I.state)) r Sim (L, V, s)
+            (L', V', write_moves xl yl s').
+Proof.
+  intros SIM Def Disj Uniq.
+  length_equify. general induction Len.
+  - simpl in *. eapply (SIM ∅); eauto.
+  - simpl in *; dcr.
+    edestruct Def; [cset_tac|].
+    pone_step_right; simpl. rewrite <- H1.
+    eapply IHLen; intros; eauto using injective_on_incl with cset.
+    eapply (SIM D).
+    rewrite <- update_unique_commute_eq; simpl; eauto with len.
+    erewrite lookup_list_agree; eauto.
+    symmetry. eapply agree_on_update_dead; eauto.
+    eapply disj_not_in.
+    eapply disj_1_incl. eapply disj_2_incl; eauto with cset.
+    eauto with cset.
+    rewrite H1; eapply defined_on_update_some;
+      eauto using defined_on_incl with cset.
+Qed.
+
+Lemma sim_I k Λ ZL LV VD r L L' V V' G R M s lv sl ib
+  : let nlv := reconstr_live_do_spill slot Λ ZL G s sl in
+    agree_on eq (getAnn nlv ∩ R) V V'
+    -> agree_on eq (getAnn nlv ∩ M) V (fun x => V' (slot x))
+  -> live_sound Imperative ZL LV s lv
+  -> spill_sound k ZL Λ (R,M) s sl
+  -> spill_live VD sl lv
+  -> injective_on VD slot
+  -> defined_on (R ∪ map slot M) V'
+  -> getSp sl ∪ getL sl ⊆ VD
+  -> labenv_sim Sim (sim r) SR (zip pair Λ ZL) L L'
+  -> sim r Sim (L, V, s) (L', V', do_spill slot s sl ib).
+Proof.
+  simpl. unfold reconstr_live_do_spill. unfold sim. revert_except s.
+  time (sind s).
+  intros ? ? ? ? ? ? ? ? ? ? ? ? ? ? ? ? Agr1 Agr2 LS SLS SL Inj Def Incl LSim.
+  rewrite do_spill_extract_writes.
+  exploit L_sub_SpM; eauto.
+  exploit Sp_sub_R; eauto.
+  eapply sim_write_moves; try rewrite of_list_elements; eauto with len.
+  intros ? ? Agr3.
+  eapply sim_write_moves; try rewrite of_list_elements; eauto with len.
+  intros ? ? Agr4.
+  - admit.
+  - admit.
+  - admit.
+  - admit.
+  - eauto using defined_on_incl with cset.
+  - admit.
+  - eapply injective_unique_map; eauto.
+    rewrite of_list_elements. eauto using injective_on_incl with cset.
+    admit.
+Qed.
+
+
+
+      pose proof (@update_unique_commute+ var _ (option val) _ (slot ⊝ xl) (lookup_list V xl) V' D
+                 (slot a) (V a)).
+      unfold _eq in H4. simpl in *.
+      instantiate (1:=D). hnf; intros.
+      exploit H4; eauto with len. len_simpl. rewrite lookup_list_length. eauto.
+      exploit H6; eauto.
+      Lemma option_eq_eq A
+        : forall x y, @option_eq A eq x y <-> x = y.
+      Proof.
+        split; intros; subst.
+        inv H; eauto. reflexivity.
+      Qed.
+      intros.
+      etrans
+
+      eapply H4.
+
+  Qed.
+  destruct s; simpl; intros; invt live_sound; invt spill_sound;
+        invt spill_live; simpl in * |- *).
+  - destruct e.
+    + cases. exploit H9; eauto. inv H2.
+      * eapply (sim_let_op il_statetype_I);
+          eauto 20 using op_eval_live, agree_on_update_same, agree_on_incl.
+      * case_eq (op_eval V e); intros.
+        -- pone_step_left.
+           eapply (IH s); eauto. eapply agree_on_update_dead; eauto.
+           eapply agree_on_incl; eauto.
+           rewrite <- H10. cset_tac; intuition.
+        -- pno_step_left.
+    + cases. exploit H9; eauto. inv H2.
+      * eapply (sim_let_call il_statetype_I); eauto 10 using agree_on_update_same, agree_on_incl.
+        erewrite <- omap_op_eval_live_agree; eauto. eapply agree_on_sym; eauto.
+  - eapply (sim_if_elim il_statetype_I); intros; eauto 20 using op_eval_live, agree_on_incl.
+  - eapply labenv_sim_app; eauto using zip_get.
+    + intros; simpl in *; dcr; subst.
+      split; [|split]; intros.
+      * exploit (@omap_filter_by _ _ _ _ (fun y : var => if [y \In blv] then true else false) _ _ Z0 H7);
+          eauto.
+        exploit omap_op_eval_live_agree; eauto.
+        intros. eapply argsLive_liveSound; eauto.
+        erewrite get_nth; eauto using zip_get; simpl.
+        rewrite H12. eexists; split; eauto.
+        repeat split; eauto using filter_filter_by_length.
+        eapply agree_on_incl; eauto.
+  - pno_step.
+    simpl. erewrite <- op_eval_live_agree; eauto. eapply agree_on_sym; eauto.
+  - eapply sim_fun_ptw; eauto.
+    + intros. left. rewrite <- zip_app; eauto with len. eapply IH; eauto using agree_on_incl.
+    + intros. hnf; intros; simpl in *; dcr; subst.
+      inv_get.
+      rewrite <- zip_app; eauto with len.
+      eapply IH; eauto.
+      eapply agree_on_update_filter'; eauto.
+    + hnf; intros; simpl in *; subst.
+      inv_get; simpl; eauto.
+    + eauto with len.
+    + eauto with len.
+Qed.
